Add slp first definition
In order to compute slp for CSTAR we need to annotate the command with an invariant like what is done with while loop in regular Hoare

theories/Inc.v
@@ -538,3 +538,118 @@ Proof.
 Qed.
 
 End IncSoundness.
+
+Module StrongestLiberalPostcondition.
+
+  Notation "⟦⟦ P ⟧⟧ c ⟦⟦ Q ⟧⟧" := (IncTriple P c Q) (at level 90, c at next level).
+
+  (* Strongest Liberal Postcondition for normal executions *)
+  Fixpoint slp_ok (P: assertion) (c: com) : assertion :=
+  match c with
+  | SKIP => P
+  | ERROR => ffalse
+  | ASSUME b => atrue b //\\ P
+  | ASSIGN x a => aexists (fun (m: Z) => aexists (fun (n: Z) =>
+      aequal (VAR x) n //\\ aupdate x (CONST m) (P //\\ aequal a n)))
+  | NONDET x => aforall (fun (m: aexp) => aupdate x m P)
+  | c1 ⊕ c2 => slp_ok P c1 \\// slp_ok P c2
+  | c1 ;; c2 => slp_ok (slp_ok P c1) c2
+  | CSTAR c => ffalse (* FIXME: Change IMP so that Cstar can carry invariant  *)
+  end.
+
+  (* Strongest Liberal Postcondition for error executions *)
+  Fixpoint slp_err (P: assertion) (c: com) : assertion :=
+  match c with
+  | SKIP => ffalse
+  | ERROR => P
+  | ASSUME b => ffalse
+  | ASSIGN x a => ffalse
+  | NONDET x => ffalse
+  | c1 ⊕ c2 => slp_err P c1 \\// slp_err P c2
+  | c1 ;; c2 => slp_err P c1 \\// slp_err (slp_ok P c1) c2
+  | CSTAR c => ffalse (* FIXME: Change IMP so that Cstar can carry invariant  *)
+  end.
+
+  Lemma slp_ok_correct: forall P c,
+    ⟦⟦ P ⟧⟧ c ⟦⟦ ok ↑ slp_ok P c ⟧⟧.
+  Proof.
+    intros P c. revert P.
+    induction c; intros P r HQ; cbn [slp_ok] in HQ.
+    - (* SKIP *) destruct r as [s|s]; [|contradiction].
+      exists s. split; [exact HQ | apply cexec_skip].
+    - (* ERROR *) destruct r as [s|s]; contradiction.
+    - (* ASSIGN x a *) destruct r as [s|s]; [|contradiction].
+      destruct HQ as [m [n [Heq_x [HP Heq_a]]]].
+      cbn in HP, Heq_a, Heq_x.
+      unfold aequal in Heq_x, Heq_a. cbn in Heq_x, Heq_a.
+      exists (update x m s). split; [ exact HP | ].
+      replace s with (update x (aeval a (update x m s)) (update x m s)) at 2.
+      + apply cexec_assign.
+      + rewrite Heq_a. extensionality y.
+        unfold update. destruct (string_dec x y) as [-> | Hneq].
+        * symmetry. exact Heq_x.
+        * reflexivity.
+    - (* NONDET x *) destruct r as [s|s]; [|contradiction].
+      exists (update x 0 s). split.
+      + apply (HQ (CONST 0)).
+      + replace s with (update x (s x) (update x 0 s)) at 2.
+        * apply cexec_nondet.
+        * unfold update. extensionality y.
+          destruct (string_dec x y) as [-> | _]; reflexivity.
+    - (* ASSUME b *) destruct r as [s|s]; [|contradiction].
+      destruct HQ as [Hb HP].
+      exists s. split; [exact HP | apply cexec_assume; exact Hb].
+    - (* SEQ c1 c2 *) destruct r as [s|s]; [|contradiction].
+      destruct (IHc2 (slp_ok P c1) (RNormal s) HQ) as (s_mid & HQmid & EXEC2).
+      destruct (IHc1 P (RNormal s_mid) HQmid) as (s_pre & HPpre & EXEC1).
+      exists s_pre. split; [ exact HPpre | eapply cexec_seq; eauto ].
+    - (* CHOICE c1 c2 *) destruct r as [s|s]; [|contradiction].
+      destruct HQ as [H1 | H2].
+      + destruct (IHc1 P (RNormal s) H1) as (s0 & HP & EXEC).
+        exists s0. split; [ exact HP | apply cexec_choice_left; exact EXEC ].
+      + destruct (IHc2 P (RNormal s) H2) as (s0 & HP & EXEC).
+        exists s0. split; [ exact HP | apply cexec_choice_right; exact EXEC ].
+    - (* CSTAR c *) destruct r as [s|s]; contradiction.
+  Qed.
+
+  Lemma slp_err_correct: forall P c,
+    ⟦⟦ P ⟧⟧ c ⟦⟦ err ↑ slp_err P c ⟧⟧.
+  Proof.
+    intros P c. revert P.
+    induction c; intros P r HQ; cbn [slp_err] in HQ.
+    - (* SKIP *) destruct r as [s|s]; contradiction.
+    - (* ERROR *) destruct r as [s|s]; [contradiction|].
+      exists s. split; [exact HQ | apply cexec_error].
+    - (* ASSIGN *) destruct r as [s|s]; contradiction.
+    - (* NONDET *) destruct r as [s|s]; contradiction.
+    - (* ASSUME *) destruct r as [s|s]; contradiction.
+    - (* SEQ c1 c2 *) destruct r as [s|s]; [contradiction|].
+      destruct HQ as [H1 | H2].
+      + destruct (IHc1 P (RError s) H1) as (s_pre & HP & EXEC1).
+        exists s_pre. split; [exact HP | apply cexec_seq_error; exact EXEC1].
+      + destruct (IHc2 (slp_ok P c1) (RError s) H2) as (s_mid & HQmid & EXEC2).
+        destruct (slp_ok_correct P c1 (RNormal s_mid) HQmid) as (s_pre & HP & EXEC1).
+        exists s_pre. split; [exact HP | eapply cexec_seq_error_right; eauto].
+    - (* CHOICE c1 c2 *) destruct r as [s|s]; [contradiction|].
+      destruct HQ as [H1 | H2].
+      + destruct (IHc1 P (RError s) H1) as (s0 & HP & EXEC).
+        exists s0. split; [exact HP | apply cexec_choice_left; exact EXEC].
+      + destruct (IHc2 P (RError s) H2) as (s0 & HP & EXEC).
+        exists s0. split; [exact HP | apply cexec_choice_right; exact EXEC].
+    - (* CSTAR c *) destruct r as [s|s]; contradiction.
+  Qed.
+
+  Theorem slp_correct: forall P c,
+    let Q : postassertion := fun r => match r with
+                                      | RNormal s => slp_ok  P c s
+                                      | RError  s => slp_err P c s
+                                      end in
+    ⟦⟦ P ⟧⟧ c ⟦⟦  Q ⟧⟧.
+  Proof.
+    intros P c Q r HQ. subst Q. cbn in HQ.
+    destruct r as [s | s].
+    - apply (slp_ok_correct  P c (RNormal s) HQ).
+    - apply (slp_err_correct P c (RError s) HQ).
+  Qed.
+
+End StrongestLiberalPostcondition.
